Sorting/MergeSort.v
@@ -7,22 +7,32 @@ Require Export Div2.
 Require Export Sort.
 Require Export ListLemmas.
 
+Require Import InsertionSort.
+
 Set Implicit Arguments.
 
-Fixpoint merge (A : LinDec) (l1 : list A) {struct l1} : list A -> list A :=
-    fix f (l2 : list A) {struct l2} : list A :=
-    match l1, l2 with
-        | [], _ => l2
-        | _, [] => l1
-        | h1 :: t1, h2 :: t2 =>
-            if h1 <=? h2
-            then h1 :: merge A t1 l2
-            else h2 :: f t2
-    end.
+Function merge (A : LinDec) (l : list A * list A)
+    {measure lenSum l} : list A :=
+let (l1, l2) := l in match l1, l2 with
+    | [], _ => l2
+    | _, [] => l1
+    | h :: t, h' :: t' =>
+        if h <=? h'
+        then h :: merge A (t, l2)
+        else h' :: merge A (l1, t')
+end.
+Proof.
+  intros. unfold lenSum. simpl. omega.
+  intros. unfold lenSum. simpl. omega.
+Defined.
 
-(* Mergesort using Program Fixpoint. *)
-Program Fixpoint msPF (A : LinDec) (l : list A) 
-    {measure (length l)} : list A :=
+Hint Extern 1 (length (drop _ _) < length _) =>
+  apply drop_length_lt; simpl; [omega | inversion 1].
+
+Hint Extern 1 (length (take _ _) < length _) =>
+  apply take_length_lt; apply lt_div2; simpl; omega.
+
+Function ms (A : LinDec) (l : list A) {measure length l} : list A :=
 match l with
     | [] => []
     | [x] => [x]
@@ -30,101 +40,51 @@ match l with
       let n := div2 (length l') in
       let l1 := take n l' in
       let l2 := drop n l' in
-      merge A (msPF A l1) (msPF A l2)
+      merge A (ms A l1, ms A l2)
 end.
-Next Obligation.
-  apply take_length_lt. apply lt_div2. destruct l; simpl;
-  try (contradiction H0; auto; fail); try omega. Qed.
-Next Obligation.
-  apply drop_length_lt; auto.
-    destruct l; simpl. contradiction H0; auto.
-      destruct l; simpl. contradiction (H c); auto. omega. Qed.
-Next Obligation.
-  split; repeat intro; inversion H3.
-Defined.
+Proof. all: auto. Defined.
 
-Eval compute in msPF natle testl.
+Hint Extern 1 (length _ < length _) =>
+match goal with
+    | H : context [ms_split] |- _ =>
+        try (eapply ms_split_len1; eauto; fail);
+        eapply ms_split_len2; eauto
+end.
 
-(* Mergesort using Function. *)
-Function msFun (A : LinDec) (l : list A) {measure length l} : list A :=
+Function ms2 (A : LinDec) (l : list A) {measure length l} : list A :=
 match l with
     | [] => []
     | [x] => [x]
     | l' =>
-      let n := div2 (length l') in
-      let l1 := take n l' in
-      let l2 := drop n l' in
-      merge A (msFun A l1) (msFun A l2)
+        let (l1, l2) := ms_split l' in
+          merge A (ms2 A l1, ms2 A l2)
 end.
-Proof.
-  intros. apply drop_length_lt; simpl. omega. inversion 1.
-  intros. apply take_length_lt. apply lt_div2. simpl. omega.
-Defined.
+Proof. all: auto. Defined.
 
-Eval compute in msFun natle testl.
-
-(* Mergesort using fuel recursion. *)
-Fixpoint msFuel' (A : LinDec) (n : nat) (l : list A) : list A :=
-match n, l with
-    | 0, _ => []
-    | _, [] => []
-    | _, [x] => [x]
-    | S n', l' =>
-        let n := div2 (length l') in
-        let l1 := take n l' in
-        let l2 := drop n l' in
-        merge A (msFuel' A n' l1) (msFuel' A n' l2)
+Hint Extern 1 (length _ < length _) =>
+match goal with
+    | H : (length ?l <=? S (S _)) = false |- _ =>
+        destruct l as [| ? | ? ? ?] using list_ind2;
+        simpl in H; inversion_clear H
 end.
 
-Eval compute in msFuel' natle 5 testl.
-
-(* Mergesort using well-founded recursion and refine. *)
-Definition msWfRef (A : LinDec) : list A -> list A.
-refine (Fix (@lengthOrder_wf A) _
-(fun (l : list A) =>
-match l with
-    | [] => fun _ => []
-    | [x] => fun _ => [x]
-    | x :: y :: l' => fun msWf =>
-        let n := div2 (length (x :: y :: l')) in
-        let l1 := take n (x :: y :: l') in
-        let l2 := drop n (x :: y :: l') in merge A (msWf l1 _) (msWf l2 _)
-end)).
+Function hms (n : nat) (A : LinDec) (l : list A) {measure length l}
+  : list A :=
+  if @leqb natle (length l) (S (S n))
+  then insertionSort A l
+  else  let n := Nat.div2 (length l) in
+        let l1 := take n l in
+        let l2 := drop n l in
+          merge A (hms n A l1, hms n A l2).
 Proof.
-  all: unfold l1, l2, n.
-    apply take_length_lt. apply lt_div2. simpl. omega.
-    apply drop_length_lt; simpl.
-      omega.
-      inversion 1.
+  all: auto.
 Defined.
 
-(* Mergesort using Bove-Capretta *)
-Inductive msDom {A : LinDec} : list A -> Type :=
-    | msDom0 : msDom []
-    | msDom1 : forall x : A, msDom [x]
-    | msDom2 : forall l : list A,
-        msDom (take (div2 (length l)) l) ->
-        msDom (drop (div2 (length l)) l) -> msDom l.
-
-Fixpoint msBC' {A : LinDec} {l : list A} (dom : msDom l) : list A :=
-match dom with
-    | msDom0 => []
-    | msDom1 x => [x]
-    | msDom2 l dom1 dom2 =>
-        let l1 := msBC' dom1 in
-        let l2 := msBC' dom2 in merge A l1 l2
-end.
-
-Theorem msDom_all : forall (A : LinDec) (l : list A), msDom l.
+Function hms2 (n : nat) (A : LinDec) (l : list A) {measure length l}
+  : list A :=
+  if @leqb natle (length l) (S (S n))
+  then insertionSort A l
+  else let (l1, l2) := ms_split l in merge A (hms2 n A l1, hms2 n A l2).
 Proof.
-  intro. apply well_founded_induction_type with lengthOrder.
-    apply lengthOrder_wf.
-    intros l ms. destruct l as [| h [| h' t]]; constructor.
-      apply ms. apply take_length_lt. apply lt_div2. simpl. omega.
-      apply ms. apply drop_length_lt. simpl. omega. inversion 1.
+  all: auto.
 Defined.
-
-Definition msBC (A : LinDec) (l : list A) : list A :=
-    msBC' (msDom_all A l).
-
-Eval compute in msBC natle testl.
