Sorting/MergeSortSpec.v
@@ -1,59 +1,183 @@
 Add Rec LoadPath "/home/zeimer/Code/Coq".
 
 Require Import MergeSort.
+Require Import InsertionSort.
 
 Set Implicit Arguments.
 
-(*Functional Scheme merge_ind := Induction for merge Sort Prop.*)
-
-Theorem merge_sorted : forall (A : LinDec) (l1 l2 : list A),
-    sorted A l1 -> sorted A l2 -> sorted A (merge A l1 l2).
+Theorem merge_sorted :
+  forall (A : LinDec) (l : list A * list A),
+    sorted A (fst l) -> sorted A (snd l) -> sorted A (merge A l).
 Proof.
-Admitted.
-
-Lemma merge_perm :
-  forall (A : LinDec) (l1 l2 : list A),
-    perm A (l1 ++ l2) (merge A l1 l2).
-Proof.
-Admitted.
-
-(*Lemma merge_In :
-  forall (A : LinDec) (x : A) (l1 l2 : list A),
-    In x (merge A l1 l2) <-> In x (l1 ++ l2).
-Proof.
-Admitted.
-
-Theorem msFun_In :
-  forall (A : LinDec) (x : A) (l : list A),
-    In x (msFun A l) <-> In x l.
-Proof.
-  split; functional induction msFun A l; auto; clear y; intro.
-    apply merge_In in H. apply in_app_or in H. destruct H.
-      eapply take_In. apply IHl0. assumption.
-      eapply drop_In. apply IHl1. assumption.
-    apply merge_In. apply in_or_app.
-      rewrite <- (take_drop (Nat.div2 (length l))) in H.
-      apply in_app_or in H. destruct H; auto.
-Qed.*)
-
-Theorem msFun_sorted :
-  forall (A : LinDec) (l : list A), sorted A (msFun A l).
-Proof.
-  intros. functional induction msFun A l; auto; clear y.
-  apply merge_sorted; assumption.
+  intros. functional induction merge A l; simpl in *; auto;
+  rewrite merge_equation in *.
+    destruct t; simpl in *; dec.
+    destruct t'; simpl in *; dec.
 Qed.
 
-Theorem msFun_perm :
-  forall (A : LinDec) (l : list A), perm A l (msFun A l).
+Theorem merge_perm :
+  forall (A : LinDec) (l : list A * list A),
+    perm A (fst l ++ snd l) (merge A l).
 Proof.
-  intros. functional induction msFun A l; auto; clear y.
-    rewrite <- (take_drop (Nat.div2 (length l))) at 1.
-      rewrite <- merge_perm. apply perm_app; assumption.
+  intros. functional induction merge A l; simpl; auto; try clear y.
+    rewrite app_nil_r. auto.
+    eapply perm_trans.
+      rewrite app_comm_cons. apply perm_app_comm.
+      simpl. apply perm_cons. simpl in IHl0. rewrite <- IHl0.
+        apply perm_app_comm.
 Qed.
 
-Instance Sort_msFun : Sort :=
+Theorem ms_sorted :
+  forall (A : LinDec) (l : list A), sorted A (ms A l).
+Proof.
+  intros. functional induction ms A l; auto; clear y.
+  apply merge_sorted; simpl; assumption.
+Qed.
+
+Theorem ms_perm :
+  forall (A : LinDec) (l : list A), perm A l (ms A l).
+Proof.
+  intros. functional induction ms A l; auto; clear y.
+  rewrite <- merge_perm, <- (take_drop (Nat.div2 (length l))) at 1; simpl.
+  apply perm_app; assumption.
+Qed.
+
+Instance Sort_ms : Sort :=
 {
-    sort := msFun;
-    sort_sorted := msFun_sorted;
-    sort_perm := msFun_perm;
+    sort := ms;
+    sort_sorted := ms_sorted;
+    sort_perm := ms_perm;
 }.
+
+(* Specification of ms2. *)
+Theorem ms2_sorted :
+  forall (A : LinDec) (l : list A), sorted A (ms2 A l).
+Proof.
+  intros. functional induction ms2 A l; auto; clear y.
+  apply merge_sorted; simpl; assumption.
+Qed.
+
+Fixpoint interleave {A : Type} (l1 l2 : list A) : list A :=
+match l1, l2 with
+    | [], _ => l2
+    | _, [] => l1
+    | h1 :: t1, h2 :: t2 => h1 :: h2 :: interleave t1 t2
+end.
+
+Theorem ms_split_interleave :
+  forall (A : Type) (l : list A),
+    interleave (fst (ms_split l)) (snd (ms_split l)) = l.
+Proof.
+  induction l as [| | h h' t] using list_ind2; cbn; auto.
+    destruct (ms_split t). cbn in *. rewrite IHt. auto.
+Qed.
+
+Theorem interleave_ms_split :
+  forall (A : Type) (l1 l2 : list A),
+    ms_split (interleave l1 l2) = (l1, l2).
+Proof.
+  induction l1 as [| h1 t1]. cbn.
+Abort.
+
+Lemma count_interleave :
+  forall (A : LinDec) (x : A) (l1 l2 : list A),
+    count A x (interleave l1 l2) = count A x l1 + count A x l2.
+Proof.
+  induction l1 as [| h1 t1]; cbn; auto.
+    destruct l2 as [| h2 t2]; cbn.
+      apply plus_n_O.
+      dec; rewrite IHt1; omega.
+Qed.
+
+Lemma perm_interleave :
+  forall (A : LinDec) (l1 l1' l2 l2' : list A),
+    perm A l1 l1' -> perm A l2 l2' ->
+      perm A (interleave l1 l2) (interleave l1' l2').
+Proof.
+  unfold perm. intros. rewrite !count_interleave. auto.
+Qed.
+
+Lemma merge_perm_interleave :
+  forall (A : LinDec) (l : list A * list A),
+    perm A (merge A l) (interleave (fst l) (snd l)).
+Proof.
+  unfold perm; intros. rewrite count_interleave.
+  rewrite <- merge_perm. rewrite count_app. auto.
+Qed.
+
+Theorem ms2_perm :
+  forall (A : LinDec) (l : list A), perm A l (ms2 A l).
+Proof.
+  intros. functional induction ms2 A l; auto; clear y.
+  rewrite merge_perm_interleave. simpl.
+    rewrite <- ms_split_interleave at 1. apply perm_interleave.
+      rewrite e0. simpl. auto.
+      rewrite e0. simpl. auto.
+Qed.
+
+Instance Sort_ms2 : Sort :=
+{
+    sort := ms2;
+    sort_sorted := ms2_sorted;
+    sort_perm := ms2_perm;
+}.
+
+(* Specification of hms. *)
+Theorem hms_sorted :
+  forall (n : nat) (A : LinDec) (l : list A), sorted A (hms n A l).
+Proof.
+  intros. functional induction hms n A l; auto.
+    apply (@sort_sorted Sort_insertionSort).
+    apply merge_sorted; simpl; assumption.
+Qed.
+
+Theorem hms_perm :
+  forall (n : nat) (A : LinDec) (l : list A), perm A l (hms n A l).
+Proof.
+  intros. functional induction hms n A l; auto.
+    apply (@sort_perm Sort_insertionSort).
+    rewrite <- merge_perm, <- (take_drop (Nat.div2 (length l))) at 1; simpl.
+      apply perm_app; assumption.
+Qed.
+
+Instance Sort_hms (n : nat) : Sort :=
+{
+    sort := hms n;
+    sort_sorted := hms_sorted n;
+    sort_perm := hms_perm n;
+}.
+
+(* Specification of hms2. *)
+Theorem hms2_sorted :
+  forall (n : nat) (A : LinDec) (l : list A), sorted A (hms2 n A l).
+Proof.
+  intros. functional induction hms2 n A l; auto.
+    apply (@sort_sorted Sort_insertionSort).
+    apply merge_sorted; simpl; assumption.
+Qed.
+
+Theorem hms2_perm :
+  forall (n : nat) (A : LinDec) (l : list A), perm A l (hms2 n A l).
+Proof.
+  intros. functional induction hms2 n A l; auto.
+    apply (@sort_perm Sort_insertionSort).
+    rewrite merge_perm_interleave. simpl.
+      rewrite <- ms_split_interleave at 1. apply perm_interleave.
+        rewrite e0. simpl. auto.
+        rewrite e0. simpl. auto.
+Qed.
+
+Instance Sort_hms2 (n : nat) : Sort :=
+{
+    sort := hms2 n;
+    sort_sorted := hms2_sorted n;
+    sort_perm := hms2_perm n;
+}.
+
+(* TODO *) Lemma ms2_is_ms :
+  forall (A : LinDec) (l : list A), ms2 A l = ms A l.
+Proof.
+  intros. functional induction ms2 A l; auto.
+    rewrite ms_equation. destruct l as [| h [| h' t]]; inversion y.
+      rewrite IHl0, IHl1.
+Abort.
